PropositionalLogic/Complete_Intuitionistic_Kripke.v
@@ -11,13 +11,27 @@ Require Import Logic.PropositionalLogic.KripkeSemantics.
 Local Open Scope logic_base.
 Local Open Scope PropositionalLogic.
 
-Definition DCS (Var: Type): Type := sig (fun Phi =>
-  @derivable_closed _ _ (IntuitionisticPropositionalLogic.G Var) Phi /\
-  @orp_witnessed _ _ _ (IntuitionisticPropositionalLogic.G Var) Phi /\
-  consistent (IntuitionisticPropositionalLogic.G Var) Phi).
+Section Completeness.
 
-Definition canonical_frame (Var: Type): KripkeSemantics.frame.
-  refine (KripkeSemantics.Build_frame (DCS Var) (fun a b => Included _ (proj1_sig b) (proj1_sig a)) _).
+Context (Var: Type).
+Context (CV: Countable Var).
+
+Instance L: Language := PropositionalLanguage.L Var.
+Instance nL: NormalLanguage L := PropositionalLanguage.nL Var.
+Instance pL: PropositionalLanguage L := PropositionalLanguage.pL Var.
+Instance R: SyntacticReduction L := IntuitionisticReduction.
+Instance nR: NormalSyntacticReduction L R := PropositionalLanguage.nIntuitionisticReduction.
+Instance G: ProofTheory L := IntuitionisticPropositionalLogic.G Var.
+Instance mpG: MinimunPropositionalLogic L G := IntuitionisticPropositionalLogic.mpG Var.
+Instance ipG: IntuitionisticPropositionalLogic L G := IntuitionisticPropositionalLogic.ipG Var.
+
+Definition DCS: Type := sig (fun Phi =>
+  derivable_closed Phi /\
+  orp_witnessed Phi /\
+  consistent Phi).
+
+Definition canonical_frame: KripkeSemantics.frame.
+  refine (KripkeSemantics.Build_frame DCS (fun a b => Included _ (proj1_sig b) (proj1_sig a)) _).
   constructor.
   + hnf; intros.
     hnf; intros; auto.
@@ -25,56 +39,56 @@ Definition canonical_frame (Var: Type): KripkeSemantics.frame.
     hnf; intros; auto.
 Defined.
 
-Program Definition canonical_eval (Var: Type): Var -> KripkeSemantics.sem (canonical_frame Var) :=
+Program Definition canonical_eval: Var -> KripkeSemantics.sem canonical_frame :=
   fun p a => a (PropositionalLanguage.varp p).
 Next Obligation.
   apply H; auto.
 Qed.
 
-Definition canonical_model {Var: Type} (Phi: DCS Var): @model _ (KripkeSemantics.SM Var) :=
-  KripkeSemantics.Build_model Var (canonical_frame Var) (canonical_eval Var) Phi.
+Definition canonical_model (Phi: DCS): @model _ (KripkeSemantics.SM Var) :=
+  KripkeSemantics.Build_model Var canonical_frame canonical_eval Phi.
 
-Lemma Lindenbaum_lemma {Var: Type}: Countable Var ->
+Lemma Lindenbaum_lemma:
   forall Phi x,
-    ~ @derivable _ (IntuitionisticPropositionalLogic.G Var) Phi x ->
+    ~ Phi |-- x ->
     exists Psi,
       Included _ Phi Psi /\
-      ~ @derivable _ (IntuitionisticPropositionalLogic.G Var) Psi x /\
-      @derivable_closed _ _ (IntuitionisticPropositionalLogic.G Var) Psi /\
-      @orp_witnessed _ _ _ (IntuitionisticPropositionalLogic.G Var) Psi /\
-      consistent (IntuitionisticPropositionalLogic.G Var) Psi.
+      ~ Psi |-- x /\
+      derivable_closed Psi /\
+      orp_witnessed Psi /\
+      consistent Psi.
 Proof.
   intros.
-  apply PropositionalLanguage.formula_countable in X.
+  assert (Countable expr) by (apply PropositionalLanguage.formula_countable; auto).
   set (step :=
           fun n Phi x0 =>
              Phi x0 \/
             (inj_R _ _ X x0 n /\
-             ~ @derivable _ (IntuitionisticPropositionalLogic.G Var) (Union _ Phi (Singleton _ x0)) x)).
+             ~ (Union _ Phi (Singleton _ x0)) |-- x)).
   exists (LindenbaumConstruction step Phi).
   assert (Included expr Phi (LindenbaumConstruction step Phi) /\
-          ~ @derivable _ (IntuitionisticPropositionalLogic.G Var) (LindenbaumConstruction step Phi) x /\
-          (~ @derivable _ (IntuitionisticPropositionalLogic.G Var) (LindenbaumConstruction step Phi) x ->
-           @derivable_closed _ _ (IntuitionisticPropositionalLogic.G Var) (LindenbaumConstruction step Phi)) /\
-          (~ @derivable _ (IntuitionisticPropositionalLogic.G Var) (LindenbaumConstruction step Phi) x ->
-           @orp_witnessed _ _ _ (IntuitionisticPropositionalLogic.G Var) (LindenbaumConstruction step Phi))).
+          ~ LindenbaumConstruction step Phi |-- x /\
+          (~ LindenbaumConstruction step Phi |-- x ->
+           derivable_closed (LindenbaumConstruction step Phi)) /\
+          (~ LindenbaumConstruction step Phi |-- x ->
+           orp_witnessed (LindenbaumConstruction step Phi))).
   Focus 2. {
     destruct H0 as [? [? [? ?]]].
     split; [| split; [| split; [| split]]]; auto.
     intro; apply H1.
-    pose proof @falsep_elim_derivable _ _ _ _ _ _ (IntuitionisticPropositionalLogic.ipG Var) (LindenbaumConstruction step Phi) x.
-    eapply (@derivable_modus_ponens _ _ _ _ _ (IntuitionisticPropositionalLogic.mpG Var) (LindenbaumConstruction step Phi)); [exact H4 | exact H5].
+    pose proof falsep_elim_derivable (LindenbaumConstruction step Phi) x.
+    eapply derivable_modus_ponens; [exact H4 | exact H5].
   } Unfocus.
   split; [| split; [| split]].
   + apply (Lindenbaum_spec_included _ _ 0).
   + apply (Lindenbaum_spec_pos _ _
-            (fun xs => @provable _ (IntuitionisticPropositionalLogic.G Var) (multi_imp xs x))
-            (fun Phi => @derivable _ (IntuitionisticPropositionalLogic.G Var) Phi x)).
+            (fun xs => |-- multi_imp xs x)
+            (fun Phi => Phi |-- x)).
     - intros; apply derivable_provable.
     - intros ? ? ? ?; left; auto.
     - apply H.
     - intros.
-      destruct (Classical_Prop.classic (exists x0, inj_R _ _ X x0 n /\ ~ @derivable _ (IntuitionisticPropositionalLogic.G Var) (Union _ S (Singleton _ x0)) x)) as [[x0 [? ?]] |].
+      destruct (Classical_Prop.classic (exists x0, inj_R _ _ X x0 n /\ ~ (Union _ S (Singleton _ x0)) |-- x)) as [[x0 [? ?]] |].
       * intro; apply H2; clear H2.
         eapply derivable_weaken; [| exact H3].
         hnf; intros ? [? | [? ?]]; [left; auto |].
@@ -92,9 +106,9 @@ Proof.
     unfold step at 1.
     right; split; auto.
     intro.
-    rewrite (@deduction_theorem _ _ _ _ _ (IntuitionisticPropositionalLogic.mpG Var)) in H3.
+    rewrite deduction_theorem in H3.
     eapply derivable_weaken in H3; [| apply (Lindenbaum_spec_included _ _ n)].
-    pose proof @derivable_modus_ponens _ _ _ _ _ (IntuitionisticPropositionalLogic.mpG Var) _ _ _ H1 H3.
+    pose proof derivable_modus_ponens _ _ _ H1 H3.
     auto.
   + intros; hnf; intros x0 y0 ?.
     destruct (im_inj _ _ X x0) as [nx ?].
@@ -103,28 +117,29 @@ Proof.
       [| destruct HH as [HH | HH]; apply Lindenbaum_spec_neg in HH; auto].
     simpl.
     unfold step at 1 3.
-    assert (~ @derivable _ (IntuitionisticPropositionalLogic.G Var) (Union _ (LindenbaumChain step Phi nx) (Singleton _ x0)) x \/ ~ @derivable _ (IntuitionisticPropositionalLogic.G Var) (Union _ (LindenbaumChain step Phi ny) (Singleton _ y0)) x) as HH;
+    assert (~ Union _ (LindenbaumChain step Phi nx) (Singleton _ x0) |-- x \/
+            ~ Union _ (LindenbaumChain step Phi ny) (Singleton _ y0) |-- x) as HH;
       [| destruct HH as [HH | HH]; auto].
     apply Classical_Prop.not_and_or; intros [? ?].
-    rewrite (@deduction_theorem _ _ _ _ _ (IntuitionisticPropositionalLogic.mpG Var)) in H4, H5.
+    rewrite deduction_theorem in H4, H5.
     eapply derivable_weaken in H4; [| apply (Lindenbaum_spec_included _ _ nx)].
     eapply derivable_weaken in H5; [| apply (Lindenbaum_spec_included _ _ ny)].
-    pose proof @orp_elim_derivable _ _ _ _ _ _ (IntuitionisticPropositionalLogic.ipG Var) (LindenbaumConstruction step Phi) x0 y0 x.
-    pose proof @derivable_modus_ponens _ _ _ _ _ (IntuitionisticPropositionalLogic.mpG Var) _ _ _ H4 H6.
-    pose proof @derivable_modus_ponens _ _ _ _ _ (IntuitionisticPropositionalLogic.mpG Var) _ _ _ H5 H7.
-    apply (@derivable_assum _ _ _ _ _ (IntuitionisticPropositionalLogic.mpG Var) _ (x0 || y0)) in H1.
-    pose proof @derivable_modus_ponens _ _ _ _ _ (IntuitionisticPropositionalLogic.mpG Var) _ _ _ H1 H8.
+    pose proof orp_elim_derivable (LindenbaumConstruction step Phi) x0 y0 x.
+    pose proof derivable_modus_ponens _ _ _ H4 H6.
+    pose proof derivable_modus_ponens _ _ _ H5 H7.
+    apply (derivable_assum _ (x0 || y0)) in H1.
+    pose proof derivable_modus_ponens _ _ _ H1 H8.
     auto.
 Qed.
 
-Lemma truth_lemma {Var: Type} {CV: Countable Var}: forall (Phi: DCS Var) x, canonical_model Phi |= x <-> proj1_sig Phi x.
+Lemma truth_lemma: forall (Phi: DCS) x, canonical_model Phi |= x <-> proj1_sig Phi x.
 Proof.
   intros.
   revert x.
-  pose proof (fun Phi: DCS Var => @derivable_closed_element_derivable _ _ _ _ _ (IntuitionisticPropositionalLogic.mpG Var) (proj1_sig Phi) (proj1 (proj2_sig Phi))).
+  pose proof (fun Phi: DCS => derivable_closed_element_derivable (proj1_sig Phi) (proj1 (proj2_sig Phi))).
   pose proof @KripkeSemantics.intuitionistic_consistent Var.
-  pose proof @intuitionistic_reduction_consistent _ _ _ _  _ _ (IntuitionisticPropositionalLogic.ipG Var).
-  apply (@truth_lemma_from_syntactic_reduction  _ _ (PropositionalLanguage.nIntuitionisticReduction) _ _ H1 H0 _ _ (H Phi)).
+  pose proof intuitionistic_reduction_consistent.
+  apply (truth_lemma_from_syntactic_reduction _ _ _ H1 H0 _ _ (H Phi)).
   intros.
   clear H0 H1.
   revert Phi.
@@ -132,14 +147,14 @@ Proof.
   + destruct H2.
     specialize (IHx1 H0 Phi).
     specialize (IHx2 H1 Phi).
-    pose proof @DCS_andp_iff _ _ _ _ _ _ (IntuitionisticPropositionalLogic.ipG Var) (proj1_sig Phi) (proj1 (proj2_sig Phi)) x1 x2.
+    pose proof DCS_andp_iff (proj1_sig Phi) (proj1 (proj2_sig Phi)) x1 x2.
     simpl in *.
     unfold KripkeSemantics.sem_and.
     tauto.
   + destruct H2.
     specialize (IHx1 H0 Phi).
     specialize (IHx2 H1 Phi).
-    pose proof @DCS_orp_iff _ _ _ _ _ _ (IntuitionisticPropositionalLogic.ipG Var) (proj1_sig Phi) (proj1 (proj2_sig Phi)) (proj1 (proj2 (proj2_sig Phi))) x1 x2.
+    pose proof DCS_orp_iff (proj1_sig Phi) (proj1 (proj2_sig Phi)) (proj1 (proj2 (proj2_sig Phi))) x1 x2.
     simpl in *.
     unfold KripkeSemantics.sem_or.
     tauto.
@@ -151,15 +166,15 @@ Proof.
       rewrite H.
       apply (@deduction_theorem _ _ _ _ _ (IntuitionisticPropositionalLogic.mpG Var)).
       apply Classical_Prop.NNPP; intro.
-      pose proof Lindenbaum_lemma CV _ _ H3.
+      pose proof Lindenbaum_lemma _ _ H3.
       destruct H4 as [Psi [? [? ?]]].
       hnf in H2.
       specialize (H2 (exist _ Psi H6)).
       assert (Included _ (proj1_sig Phi) Psi) by (hnf; intros; apply H4; left; auto).
       specialize (H2 H7).
       simpl in IHx1, IHx2.
-      change (KripkeSemantics.model_frame (canonical_model Phi)) with (canonical_frame Var) in H2.
-      change (KripkeSemantics.model_var (canonical_model Phi)) with (canonical_eval Var) in H2.
+      change (KripkeSemantics.model_frame (canonical_model Phi)) with canonical_frame in H2.
+      change (KripkeSemantics.model_var (canonical_model Phi)) with canonical_eval in H2.
       rewrite IHx1, IHx2 in H2; simpl in H2.
       assert (Psi x1) by (apply H4; right; constructor).
       specialize (H2 H8).
@@ -167,16 +182,16 @@ Proof.
       rewrite H in H2; auto.
     - intros.
       hnf; intros Psi ?H.
-      change (DCS Var) in Psi.
+      change DCS in Psi.
       simpl in H3.
-      change (KripkeSemantics.model_frame (canonical_model Phi)) with (canonical_frame Var).
-      change (KripkeSemantics.model_var (canonical_model Phi)) with (canonical_eval Var).
+      change (KripkeSemantics.model_frame (canonical_model Phi)) with canonical_frame.
+      change (KripkeSemantics.model_var (canonical_model Phi)) with canonical_eval.
       simpl in IHx1, IHx2.
       rewrite IHx1, IHx2.
       intros.
       rewrite H in H2, H4 |- *.
       eapply derivable_weaken in H2; [| exact H3].
-      exact (@derivable_modus_ponens _ _ _ _ _ (IntuitionisticPropositionalLogic.mpG Var) _ _ _ H4 H2).
+      eapply derivable_modus_ponens; [exact H4 | exact H2].
   + simpl.
     split; [intros [] | intros].
     rewrite H in H0.
@@ -188,7 +203,7 @@ Proof.
     tauto.
 Qed.
 
-Theorem complete_intuitionistic_kripke (Var: Type) (CV: Countable Var): strongly_complete (IntuitionisticPropositionalLogic.G Var) (KripkeSemantics.SM Var).
+Theorem complete_intuitionistic_kripke: strongly_complete (IntuitionisticPropositionalLogic.G Var) (KripkeSemantics.SM Var).
 Abort.
 (*
 Proof.
@@ -225,3 +240,5 @@ Proof.
 Qed.
 
 *)
+
+End Completeness.
