PropositionalLogic/IntuitionisticPropositionalLogic.v
@@ -135,9 +135,14 @@ Section IntuitionisticPropositionalLogic.
 
 Context (Var: Type).
 
-Inductive provable: @expr (PropositionalLanguage.L Var) -> Prop :=
-| syntactic_reduction_rule1: forall x y, @reduce _ IntuitionisticReduction x y -> provable x -> provable y
-| syntactic_reduction_rule2: forall x y, @reduce _ IntuitionisticReduction x y -> provable y -> provable x
+Instance L: Language := PropositionalLanguage.L Var.
+Instance nL: NormalLanguage L := PropositionalLanguage.nL Var.
+Instance pL: PropositionalLanguage L := PropositionalLanguage.pL Var.
+Instance R: SyntacticReduction L := IntuitionisticReduction.
+
+Inductive provable: expr -> Prop :=
+| syntactic_reduction_rule1: forall x y, reduce x y -> provable x -> provable y
+| syntactic_reduction_rule2: forall x y, reduce x y -> provable y -> provable x
 | modus_ponens: forall x y, provable (x --> y) -> provable x -> provable y
 | axiom1: forall x y, provable (x --> (y --> x))
 | axiom2: forall x y z, provable ((x --> y --> z) --> (x --> y) --> (x --> z))
@@ -149,12 +154,12 @@ Inductive provable: @expr (PropositionalLanguage.L Var) -> Prop :=
 | orp_elim: forall x y z, provable ((x --> z) --> (y --> z) --> (x || y --> z))
 | falsep_elim: forall x, provable (FF --> x).
 
-Instance AG: AxiomaticProofTheory.AxiomaticProofTheory (PropositionalLanguage.L Var) :=
-  AxiomaticProofTheory.Build_AxiomaticProofTheory (PropositionalLanguage.L Var) provable.
+Instance AG: AxiomaticProofTheory.AxiomaticProofTheory L :=
+  AxiomaticProofTheory.Build_AxiomaticProofTheory L provable.
 
-Instance G: ProofTheory (PropositionalLanguage.L Var) := AxiomaticProofTheory.G AG.
+Instance G: ProofTheory L := AxiomaticProofTheory.G AG.
 
-Instance mpG: MinimunPropositionalLogic (PropositionalLanguage.L Var) G.
+Instance mpG: MinimunPropositionalLogic L G.
 Proof.
   constructor.
   + apply modus_ponens.
@@ -162,7 +167,7 @@ Proof.
   + apply axiom2.
 Qed.
 
-Instance ipG: IntuitionisticPropositionalLogic (PropositionalLanguage.L Var) G.
+Instance ipG: IntuitionisticPropositionalLogic L G.
 Proof.
   constructor.
   + split.
