Makefile
@@ -11,4 +11,4 @@ all: Wf.vo base.vo IPC.vo trivial.vo Kripke.vo enumerate.vo LogicBase.vo Syntact
      PropositionalLogic/Syntax.vo PropositionalLogic/ClassicalPropositionalLogic.vo \
      PropositionalLogic/TrivialSemantics.vo PropositionalLogic/Sound_Classical_Trivial.vo \
      PropositionalLogic/Complete_Classical_Trivial.vo lib/Coqlib.vo \
-     lib/Bijection.vo lib/Countable.vo
+     lib/Bijection.vo lib/Countable.vo PropositionalLogic/Complete_Intuitionistic_Kripke.vo 
